Flapjack.lean
@@ -142,6 +142,7 @@ import Flapjack.CrepeContextBounds
 import Flapjack.Pancake.PanToCrep.Compile
 import Flapjack.Pancake.PanToCrep.ExpHdlExact
 import Flapjack.Pancake.PanToCrep.ContextExact
+import Flapjack.Pancake.PanToCrep.ContextBridge
 import Flapjack.Pancake.Proofs.CrepArith
 import Flapjack.Pancake.Proofs.CrepInline
 import Flapjack.CompileFunctionDistinct
